deps/poulet4/lib/P4cub/V1model.v
@@ -17,7 +17,10 @@ Definition externs : ToGCL.model :=
   [("_", [("mark_to_drop",  G.GAssign (E.TBit (BinNat.N.of_nat 9)) "standard_metadata.egress_spec" (BV.bit (Some 9) 511));
          ("clone3", G.GSkip);
          ("assert", G.GAssert (F.LVar "check"));
-         ("hash", G.GSkip)]);
+         ("hash", G.GSkip);
+         ("truncate", G.GSkip)
+   ]);
+  ("counter", [("count", G.GSkip)]);
   ("register", [("read", G.GSkip); ("write", G.GSkip)])
   ].
 
